skeleton

Library/Model/Model.dfy
@@ -18,6 +18,10 @@ module Model {
     Monad.Deconstruct(s)
   }
 
+  function UnifModel(n: nat): Hurd<nat> {
+    Unif.ProbUnif(n)
+  }
+
   function UniformModel(n: nat): Hurd<nat> 
     requires 0 < n 
   {
